\documentclass[a4paper, english, headtopline=0.08em, headsepline=0.04em, left = 1cm, right = 1cm, DIV=15]{article}

\input{imports}
\input{shorts}
% template from https://latex.tum.de/project/618c4a584a8e454c5f4cfa1a
\begin{document}
{
    \begin{titlepage}
    	\centering
    	\vfill
    	{\scshape\LARGE Technische Universität München \par}
    	\vfill
    	{\scshape\Large Summary of the lecture MA4800\\   \par}
    	{\huge\bfseries Foundations in Data Analysis \par}
    	\vfill
    	{\Large\itshape Instructors: Dr. Anna Veselovska and  Felix Krahmer\par}
    	\vfill
    \end{titlepage}
}

\tableofcontents
\clearpage 

%%%%% section start %%%%%%%%%
\section{Linear Algebra Review}


\begin{itemize}
	\item We work on $\mathbb{K} \in\{\mathbb{R}, \mathbb{C}\}$.
	\item $A^H = \overline{(A^T)}$.
	\item A Hermitian matrix $A$ satisfies $A=A^H$.
	\item $A^{(i)}$ are rows and $A_{(j)}$ are the columns.
	\item $A^{(i)}=\left(a_{i j}\right)_{j \in J}$ and $A_{(j)}=\left(a_{i j}\right)_{i \in I}=\left(A^{T}\right)^{(j)}$
	\item The matrix-vector product between $A \in \mathbb{K}^{I \times J}$ and $x \in \mathbb{K}^{I}$ results in the vector in $A x \in K^{\prime}$ with entries

\end{itemize}

\subsection{Matrices}

\begin{align*}
	(A x)_{i}=\sum_{j \in J} a_{i j} x_{j} .
\end{align*}
\subsection{Matrix Multiplication}
The matrix-matrix product between $A \in \mathbb{K}^{I\times J}$ and $B \in \mathbb{K}^{J \times L}$ yields the matrix in $\mathbb{K}^{I \times L}$ with entries
\begin{align*}
	(A B)_{i \ell}=\sum_{j \in J} A_{i j} B_{j \ell} .
\end{align*}
%%%%% section end %%%%%%%%%


%%%%% section start %%%%%%%%%
\section{The Singular Value Decomposition}

\subsection{The Power Method}
\begin{lemma}
Let $x \in \mathbb{R}^{d}$ be a unit $d$-dimensional vector of components $x=$ $\left(x_{1}, \ldots, x_{d}\right)$ with respect to the canonical basis and picked uniformly at random from the sphere $\left\{x:\|x\|_{2}=1\right\}$. The probability that $\left|x_{1}\right| \geq \alpha>0$ is at least $1-C \alpha \sqrt{d}$ for some absolute constant.
\end{lemma}
\subsection*{Proof}
We want the probability of y picked uniformly at random from
\begin{align*}
	B^d(1)=\left\{y\in\RR^d,||y||_2 \leq 1\right\}
\end{align*}	
satisfies $|y_1|>\alpha$. In other words, we are looking for the fraction of $B^d(1)$ that satisfies $|y_1|>\alpha$.
This corresponds to
\begin{align*}
	V_{\alpha}:=\text{Vol}(B^d(1) \cap \{y : |y_1| \leq \alpha\})
\end{align*}
\begin{align*}
	=\int_{y\in B^d(1) \cap \{y : |y_1| \leq \alpha\}}1dy
\end{align*}
\begin{align*}
	=\int_{-\alpha}^{\alpha} \left(\int_{\RR^{d-1}} 1_{y_2^2+...+y_d^2\leq 1-y_1^2}\,dy_2...dy_d\right)dy_1
\end{align*}
\begin{align*}
=\int_{-\alpha}^{\alpha} \text{Vol}\left(B^{d-1}\left(\sqrt{1-y_1^2}\right)\right)dy_1
\end{align*}
Replacing $\text{Vol}\left(B^{d-1}\left(\sqrt{1-y_1^2}\right)\right)$ with $(\sqrt{1-y_1^2})^{d-1}\text{Vol}\left(B^{d-1}(1)\right)$ since the volume the unit ball with a factor proportional to radius in the power of $d-1$.
\begin{align*}
	=\int_{-\alpha}^{\alpha} (\sqrt{1-y_1^2})^{d-1}\text{Vol}\left(B^{d-1}(1)\right)dy_1
\end{align*}
\begin{align*}
	=\text{Vol}\left(B^{d-1}(1)\right)\int_{-\alpha}^{\alpha} (1-y_1^2)^{(d-1)/2}dy_1
\end{align*}
In the integral part, $\int_{-\alpha}^{\alpha} (1-y_1^2)^{(d-1)/2}dy_1$, notice that $(1-y_1^2)^{(d-1)/2}<1$ in the whole integration domain.
Thus we can write
\begin{align*}
	=\text{Vol}\left(B^{d-1}(1)\right)\int_{-\alpha}^{\alpha} (1-y_1^2)^{(d-1)/2}dy_1
\end{align*}
\begin{align*}
	\leq \text{Vol}\left(B^{d-1}(1)\right)\int_{-\alpha}^{\alpha} 1dy_1
\end{align*}
\begin{align*}
	=2\alpha \text{Vol}\left(B^{d-1}(1)\right)
\end{align*}
Recall that volume of unit ball in d dimensions is asymptotically
\begin{align*}
	V_1 = \frac{1}{\sqrt{d\pi}}\left(\frac{2 \pi e}{d}\right)^{d/2}
\end{align*}
Hence the probability $p$ we are interested in satisfies asymptotically
\begin{align*}
	p=\frac{V_\alpha}{V_1} \propto
\frac{2\alpha\frac{1}{\sqrt{(d-1)\pi}}\left(\frac{2 \pi e}{d-1}\right)^{(d-1)/2}}
 {\frac{1}{\sqrt{d\pi}}\left(\frac{2 \pi e}{d}\right)^{d/2}}
=
\frac{2\alpha\frac{1}{\sqrt{(d-1)\pi}}\left(\frac{2 \pi e}{d-1}\right)^{(d-1)/2}}
{\frac{1}{\sqrt{d\pi}}\left(\frac{2 \pi e}{d}\right)^{(d-1)/2}\left(\frac{2 \pi e}{d}\right)^{1/2}}
\end{align*}
We simplify the last term
\begin{align*}
	=2\alpha* \left(\frac{d}{d-1}\right)^{1/2} *   \left(\frac{d}{d-1}\right)^{(d-1)/2} * \left(\frac{d}{2\pi e}\right)^{1/2}
\end{align*}
\begin{align*}
	=2\alpha*  \left(\frac{d}{\sqrt{2\pi e (d-1)}}\right) *   \left(\frac{d}{d-1}\right)^{(d-1)/2}
\end{align*}
 Since $\frac{d}{d-1} = 1+\frac{1}{d-1}$
\begin{align*}
	=2\alpha*  \left(\frac{d}{\sqrt{2\pi e (d-1)}}\right) *   \left(1+\frac{1}{d-1}\right)^{(d-1)/2}
\end{align*}
We modify the power of the same term, to show it as
\begin{align*}
	=2\alpha*  \left(\frac{d}{\sqrt{2\pi e (d-1)}}\right) *   \left(\left(1+\frac{1}{d-1}\right)^{(d-1)}\right)^{1/2}
\end{align*}
Recall that 
\begin{align*}
	e = \lim_{n \rightarrow \infty} \left(1+1/n\right)^n
\end{align*}
Thus this term is bounded with $\sqrt{e}$
\begin{align*}
	\leq 2\alpha*  \left(\frac{d}{\sqrt{2\pi e (d-1)}}\right) *   \sqrt{e}
\end{align*}
We reformulate as
\begin{align*}
	= \alpha \sqrt{d}\sqrt{\frac{2d}{\pi(d-1)}}
\end{align*}
Since $\sqrt{\frac{d}{d-1}}\leq 2$ for $d\geq 2$
\begin{align*}
	\leq \frac{2\sqrt{2}}{\pi}\alpha \sqrt{d} 
\end{align*}
Given that all of this only holds asymptotically; we might need another multiplicative constant to make it hold in general. Hence the constant $C$ in the theorem.
\begin{align*}
	p \leq  C\alpha \sqrt{d}
\end{align*}
\end{document}

%%%%% section end %%%%%%%%%